src/tls/Connection.fst
@@ -1,9 +1,10 @@
 module Connection
+module HS = FStar.HyperStack //Added automatically
 
 // Connections are top-level instances of TLS clients and servers
 
 open FStar.Heap
-open FStar.HyperHeap
+
 open FStar.HyperStack
 // JP: please stop using opening so much stuff in scope srsly
 open FStar.Seq
@@ -22,8 +23,8 @@ open Range
 open Epochs
 open Handshake
 
-module MR = FStar.Monotonic.RRef
-module HH = FStar.HyperHeap
+
+
 
 // using also Range, DataStream, TLSFragment, Record
 
@@ -57,7 +58,7 @@ let string_of_halfState = function
 let string_of_state (r,w) =
   string_of_halfState r^"/"^string_of_halfState w
 
-type c_rgn = r:TLSConstants.rgn { HH.disjoint r TLSConstants.tls_region } 
+type c_rgn = r:TLSConstants.rgn { HS.disjoint r TLSConstants.tls_region } 
 
 (*
  * AR: changing the type of state from rref to ref, with region captured in the refinement.
