src/tls/KEF.ODH.fst
@@ -2,7 +2,7 @@
 module KDF.Expand
 
 open FStar.Heap
-open FStar.HyperHeap
+
 open FStar.HyperStack
 
 open Platform.Bytes
@@ -12,8 +12,8 @@ open TLSConstants
 open TLSInfo
 
 module MM = FStar.Monotonic.Map
-module MR = FStar.Monotonic.RRef
-module HH = FStar.HyperHeap
+
+
 module HS = FStar.HyperStack
 
 assume val ideal_Expand : bool
